# baseURI: http://www.fundontology.com/InvestorAdviserAct
# imports: http://www.fundontology.com/FundRegulation

@prefix dc: <http://purl.org/dc/elements/1.1/> .
@prefix dct: <http://purl.org/dc/terms/> .
@prefix fo-fr: <http://www.fundontology.com/FundRegulation#> .
@prefix fo-iaa: <http://www.fundontology.com/InvestorAdviserAct#> .
@prefix owl: <http://www.w3.org/2002/07/owl#> .
@prefix rdf: <http://www.w3.org/1999/02/22-rdf-syntax-ns#> .
@prefix rdfs: <http://www.w3.org/2000/01/rdf-schema#> .
@prefix skos: <http://www.w3.org/2004/02/skos/core#> .
@prefix sm: <http://www.omg.org/techprocess/ab/SpecificationMetadata/> .
@prefix sp: <http://spinrdf.org/sp#> .
@prefix spin: <http://spinrdf.org/spin#> .
@prefix xsd: <http://www.w3.org/2001/XMLSchema#> .

fo-fr:Legal_Rule
  rdfs:subClassOf [
      rdf:type owl:Restriction ;
      owl:onProperty fo-fr:applies_legal ;
      owl:someValuesFrom fo-fr:Legal_Consequence ;
    ] ;
.
fo-fr:Rule_Def_US_IAA_Sect_202a11
  fo-fr:applies_legal fo-iaa:inclusion_US_IAA_Section_202_1_11 ;
.
fo-fr:Rule_Def_US_IAA_Sect_202a11_1_business
  fo-fr:applies_legal fo-iaa:inclusion_US_IAA_Section_202_1_11 ;
.
fo-fr:Rule_Def_US_IAA_Sect_202a11_1_compensation
  fo-fr:applies_legal fo-iaa:inclusion_US_IAA_Section_202_1_11 ;
.
fo-fr:Rule_Def_US_IAA_Sect_202a11_1_service
  fo-fr:applies_legal fo-iaa:inclusion_US_IAA_Section_202_1_11 ;
.
fo-fr:Rule_Excl_US_IAA_Sect_202a11_1
  fo-fr:applies_legal fo-iaa:inclusion_US_IAA_Section_202_1_11 ;
.
fo-fr:Rule_Excl_US_IAA_Sect_202a11_1_A_bank
  fo-fr:applies_legal fo-iaa:inclusion_US_IAA_Section_202_1_11 ;
.
<http://www.fundontology.com/InvestorAdviserAct>
  rdf:type owl:Ontology ;
  owl:imports <http://www.fundontology.com/FundRegulation> ;
  owl:versionInfo "Created with TopBraid Composer"^^xsd:string ;
.
fo-iaa:Defined_Ex_US_IAA_Section_202_1_11
  rdf:type owl:Class ;
  rdfs:label "Defined ex. US IAA Section 202(1)(11) business"^^xsd:string ;
  rdfs:subClassOf fo-iaa:US_IAA ;
  owl:equivalentClass [
      rdf:type owl:Class ;
      owl:intersectionOf (
          fo-iaa:Defined_Ex_US_IAA_Section_202_1_11_business
          fo-iaa:Defined_Ex_US_IAA_Section_202_1_11_service
          fo-iaa:Defined_Ex_US_IAA_Section_202_1_11_compensation
        ) ;
    ] ;
  owl:equivalentClass [
      rdf:type owl:Restriction ;
      owl:hasValue fo-iaa:Rule_Def_US_IAA_Sect_202a11 ;
      owl:onProperty fo-fr:considered_by ;
    ] ;
  skos:definition " Investment adviser” means any person who, for compensation, engages in the business of advising others, either directly or through publications or writings, as to the value of securities or as to the advisability of investing in, purchasing, or selling securities, or who, for compensation and as part of a regular business, issues or promulgates analyses or reports concerning securities."^^xsd:string ;
.
fo-iaa:Defined_Ex_US_IAA_Section_202_1_11_business
  rdf:type owl:Class ;
  rdfs:label "Defined ex. US IAA Section 202(1)(11) business"^^xsd:string ;
  rdfs:subClassOf fo-iaa:US_IAA ;
  owl:equivalentClass fo-fr:InvestmentAdviser ;
  owl:equivalentClass [
      rdf:type owl:Restriction ;
      owl:hasValue fo-iaa:Rule_Def_US_IAA_Sect_202a11_1_business ;
      owl:onProperty fo-fr:considered_by ;
    ] ;
  skos:definition " Investment adviser” means any person who, for compensation, engages in the business of advising others, either directly or through publications or writings, as to the value of securities or as to the advisability of investing in, purchasing, or selling securities, or who, for compensation and as part of a regular business, issues or promulgates analyses or reports concerning securities."^^xsd:string ;
.
fo-iaa:Defined_Ex_US_IAA_Section_202_1_11_compensation
  rdf:type owl:Class ;
  rdfs:label "Defined ex. US IAA Section 202(1)(11) compensation"^^xsd:string ;
  rdfs:subClassOf fo-iaa:US_IAA ;
  owl:equivalentClass [
      rdf:type owl:Class ;
      owl:intersectionOf (
          <http://spec.edmcouncil.org/fibo/FBC/ProductsAndServices/FinancialProductsAndServices/FinancialServiceProvider>
          [
            rdf:type owl:Restriction ;
            owl:onProperty <http://spec.edmcouncil.org/fibo/FND/Relations/Relations/provides> ;
            owl:someValuesFrom [
                rdf:type owl:Class ;
                owl:intersectionOf (
                    fo-fr:InvestmentAdvice
                    [
                      rdf:type owl:Restriction ;
                      owl:onProperty <http://spec.edmcouncil.org/fibo/FND/Relations/Relations/isClassifiedBy> ;
                      owl:someValuesFrom fo-fr:ServiceFeeType ;
                    ]
                  ) ;
              ] ;
          ]
        ) ;
    ] ;
  owl:equivalentClass [
      rdf:type owl:Restriction ;
      owl:hasValue fo-iaa:Rule_Def_US_IAA_Sect_202a11_1_compensation ;
      owl:onProperty fo-fr:considered_by ;
    ] ;
  skos:definition " Investment adviser” means any person who, for compensation, engages in the business of advising others, either directly or through publications or writings, as to the value of securities or as to the advisability of investing in, purchasing, or selling securities, or who, for compensation and as part of a regular business, issues or promulgates analyses or reports concerning securities."^^xsd:string ;
.
fo-iaa:Defined_Ex_US_IAA_Section_202_1_11_service
  rdf:type owl:Class ;
  rdfs:label "Defined ex. US IAA Section 202(1)(11) service"^^xsd:string ;
  rdfs:subClassOf fo-iaa:US_IAA ;
  owl:equivalentClass [
      rdf:type owl:Class ;
      owl:intersectionOf (
          <http://spec.edmcouncil.org/fibo/FBC/ProductsAndServices/FinancialProductsAndServices/FinancialServiceProvider>
          [
            rdf:type owl:Restriction ;
            owl:onProperty <http://spec.edmcouncil.org/fibo/FND/Relations/Relations/provides> ;
            owl:someValuesFrom fo-fr:SecuritiesAdvice ;
          ]
        ) ;
    ] ;
  owl:equivalentClass [
      rdf:type owl:Restriction ;
      owl:hasValue fo-iaa:Rule_Def_US_IAA_Sect_202a11_1_service ;
      owl:onProperty fo-fr:considered_by ;
    ] ;
  skos:definition " Investment adviser” means any person who, for compensation, engages in the business of advising others, either directly or through publications or writings, as to the value of securities or as to the advisability of investing in, purchasing, or selling securities, or who, for compensation and as part of a regular business, issues or promulgates analyses or reports concerning securities."^^xsd:string ;
.
fo-iaa:Ex_US_IAA_Section_202_1_11
  rdf:type owl:Class ;
  rdfs:label "Defined ex. US IAA Section 202(1)(11) business"^^xsd:string ;
  rdfs:subClassOf fo-iaa:US_IAA ;
  skos:definition " Investment adviser” means any person who, for compensation, engages in the business of advising others, either directly or through publications or writings, as to the value of securities or as to the advisability of investing in, purchasing, or selling securities, or who, for compensation and as part of a regular business, issues or promulgates analyses or reports concerning securities."^^xsd:string ;
.
fo-iaa:Excluded_Ex_US_IAA_Section_202_1_11
  rdf:type owl:Class ;
  sm:author "Jurgen Ziemer"^^xsd:string ;
  sm:copyright "Jayzed Data Models Inc."^^xsd:string ;
  rdfs:comment "A class to infer the Financial Service Providers that are excluded from the IAA definition of Investment Advisers."^^xsd:string ;
  rdfs:isDefinedBy <http://www.sec.gov/about/laws/iaa40.pdf> ;
  rdfs:label "Defined as Investment Adviser ex. US IAA Section 202(1)(11)"^^xsd:string ;
  rdfs:subClassOf fo-iaa:US_IAA ;
  owl:equivalentClass [
      rdf:type owl:Class ;
      owl:unionOf (
          fo-iaa:Excluded_Ex_US_IAA_Section_202_1_11_A_bank
          fo-iaa:Excluded_Ex_US_IAA_Section_202_1_11_B_professional
          fo-iaa:Excluded_Ex_US_IAA_Section_202_1_11_C_broker_dealer
          fo-iaa:Excluded_Ex_US_IAA_Section_202_1_11_D_publisher
          fo-iaa:Excluded_Ex_US_IAA_Section_202_1_11_E_gov_sec_only
          fo-iaa:Excluded_Ex_US_IAA_Section_202_1_11_F_rating_organization
        ) ;
    ] ;
  owl:equivalentClass [
      rdf:type owl:Restriction ;
      owl:hasValue fo-iaa:Rule_Excl_US_IAA_Sect_202a11 ;
      owl:onProperty fo-fr:considered_by ;
    ] ;
  skos:definition " Investment adviser” means any person who, for compensation, engages in the business of advising others, either directly or through publications or writings, as to the value of securities or as to the advisability of investing in, purchasing, or selling securities, or who, for compensation and as part of a regular business, issues or promulgates analyses or reports concerning securities."^^xsd:string ;
.
fo-iaa:Excluded_Ex_US_IAA_Section_202_1_11_A_bank
  rdf:type owl:Class ;
  rdfs:label "Excluded ex. US IAA Section 202(1)(11)(A) Bank"^^xsd:string ;
  rdfs:subClassOf fo-iaa:US_IAA ;
  owl:equivalentClass <http://spec.edmcouncil.org/fibo/FBC/FunctionalEntities/FinancialServicesEntities/DepositoryInstitution> ;
  owl:equivalentClass [
      rdf:type owl:Restriction ;
      owl:hasValue fo-iaa:Rule_Excl_US_IAA_Sect_202a11_1_A_bank ;
      owl:onProperty fo-fr:considered_by ;
    ] ;
  skos:definition """ Investment adviser exclusion (A) 
a bank, or any bank holding company as defined in the Bank Holding Company Act of 1956 [12 U.S.C. 1841 et seq.] which is not an investment company, except that the term “investment adviser” includes any bank or bank holding company to the extent that such bank or bank holding company serves or acts as an investment adviser to a registered investment company, but if, in the case of a bank, such services or actions are performed through a separately identifiable department or division, the department or division, and not the bank itself, shall be deemed to be the investment adviser;"""^^xsd:string ;
.
fo-iaa:Excluded_Ex_US_IAA_Section_202_1_11_B_professional
  rdf:type owl:Class ;
  rdfs:label "Excluded ex. US IAA Section 202(1)(11)(A) Professional"^^xsd:string ;
  rdfs:subClassOf fo-iaa:US_IAA ;
  owl:equivalentClass [
      rdf:type owl:Restriction ;
      owl:hasValue fo-iaa:Rule_Excl_US_IAA_Sect_202a11_1_B_professional ;
      owl:onProperty fo-fr:considered_by ;
    ] ;
  skos:definition """ Investment adviser exclusion (B) 
any lawyer, accountant, engineer, or teacher whose performance of such services is solely incidental to the practice of his profession;"""^^xsd:string ;
.
fo-iaa:Excluded_Ex_US_IAA_Section_202_1_11_C_broker_dealer
  rdf:type owl:Class ;
  rdfs:label "Excluded ex. US IAA Section 202(1)(11)(A) Broker/Dealer"^^xsd:string ;
  rdfs:subClassOf fo-iaa:US_IAA ;
  owl:equivalentClass <http://spec.edmcouncil.org/fibo/FBC/FunctionalEntities/FinancialServicesEntities/BrokerageFirm> ;
  owl:equivalentClass [
      rdf:type owl:Restriction ;
      owl:hasValue fo-iaa:Rule_Excl_US_IAA_Sect_202a11_1_C_broker_dealer ;
      owl:onProperty fo-fr:considered_by ;
    ] ;
  skos:definition """ Investment adviser exclusion (C) 
any broker or dealer whose performance of such services is solely incidental to the conduct of his business as a broker or dealer and who receives no special compensation therefor"""^^xsd:string ;
.
fo-iaa:Excluded_Ex_US_IAA_Section_202_1_11_D_publisher
  rdf:type owl:Class ;
  rdfs:label "Excluded ex. US IAA Section 202(1)(11)(A) Broker/Dealer"^^xsd:string ;
  rdfs:subClassOf fo-iaa:US_IAA ;
  owl:equivalentClass <http://spec.edmcouncil.org/fibo/BE/FunctionalEntities/Publishers/Publisher> ;
  owl:equivalentClass [
      rdf:type owl:Restriction ;
      owl:hasValue fo-iaa:Rule_Excl_US_IAA_Sect_202a11_1_D_publisher ;
      owl:onProperty fo-fr:considered_by ;
    ] ;
  skos:definition """ Investment adviser exclusion (D) 
the publisher of any bona fide newspaper, news magazine or business or financial publication of general and regular circulation; """^^xsd:string ;
.
fo-iaa:Excluded_Ex_US_IAA_Section_202_1_11_E_gov_sec_only
  rdf:type owl:Class ;
  rdfs:label "Excluded ex. US IAA Section 202(1)(11)(E) only US Government Securities"^^xsd:string ;
  rdfs:subClassOf fo-iaa:US_IAA ;
  owl:equivalentClass [
      rdf:type owl:Restriction ;
      owl:hasValue fo-iaa:Rule_Excl_US_IAA_Sect_202a11_1_E_gov_sec_only ;
      owl:onProperty fo-fr:considered_by ;
    ] ;
  skos:definition """ Investment adviser exclusion (E) 
any person whose advice, analyses or reports relate to no securities other than securities which are direct obligations of or obligations guaranteed as to principal or interest by the United States .."""^^xsd:string ;
.
fo-iaa:Excluded_Ex_US_IAA_Section_202_1_11_F_rating_organization
  rdf:type owl:Class ;
  rdfs:label "Excluded ex. US IAA Section 202(1)(11)(F) Rating Organization"^^xsd:string ;
  rdfs:subClassOf fo-iaa:US_IAA ;
  owl:equivalentClass <http://spec.edmcouncil.org/fibo/IND/Indicators/Indicators/FinancialInformationPublisher> ;
  owl:equivalentClass [
      rdf:type owl:Restriction ;
      owl:hasValue fo-iaa:Rule_Excl_US_IAA_Sect_202a11_1_F_rating_organization ;
      owl:onProperty fo-fr:considered_by ;
    ] ;
  skos:definition """ Investment adviser exclusion (F) 
any nationally recognized statistical rating organization"""^^xsd:string ;
.
fo-iaa:NotExcluded_Ex_US_IAA_Section_202_1_11
  rdf:type owl:Class ;
  sm:author "Jurgen Ziemer"^^xsd:string ;
  sm:copyright "Jayzed Data Models Inc."^^xsd:string ;
  rdfs:comment "A class to infer the Financial Service Providers that are excluded from the IAA definition of Investment Advisers."^^xsd:string ;
  rdfs:isDefinedBy <http://www.sec.gov/about/laws/iaa40.pdf> ;
  rdfs:label "Defined as Investment Adviser ex. US IAA Section 202(1)(11)"^^xsd:string ;
  rdfs:subClassOf fo-iaa:US_IAA ;
  owl:equivalentClass [
      rdf:type owl:Class ;
      owl:complementOf fo-iaa:Excluded_Ex_US_IAA_Section_202_1_11 ;
    ] ;
  owl:equivalentClass [
      rdf:type owl:Restriction ;
      owl:hasValue fo-iaa:Rule_Not_Excl_US_IAA_Sect_202a11 ;
      owl:onProperty fo-fr:considered_by ;
    ] ;
.
fo-iaa:Rule_Def_US_IAA_Sect_202a11
  rdf:type fo-fr:Legal_Rule ;
  fo-fr:applies_legal fo-iaa:inclusion_US_IAA_Section_202_1_11 ;
  rdfs:comment "‘‘Investment adviser’’ means any person who, for compensation, engages in the business of advising others, either directly or through publications or writings, as to the value of securities or as to the advisability of investing in, purchasing, or selling securities, or who, for compensation and as part of a regular business, issues or promulgates analyses or reports concerning securities"^^xsd:string ;
  rdfs:isDefinedBy <https://www.sec.gov/about/laws/iaa40.pdf> ;
  rdfs:label "US IAA Section 202(1)(11)"^^xsd:string ;
.
fo-iaa:Rule_Def_US_IAA_Sect_202a11_1_business
  rdf:type fo-fr:Legal_Rule ;
  fo-fr:applies_legal fo-iaa:inclusion_US_IAA_Section_202_1_11 ;
  rdfs:comment "‘‘Investment adviser’’ means any person who, for compensation, engages in the business of advising others, either directly or through publications or writings, as to the value of securities or as to the advisability of investing in, purchasing, or selling securities, or who, for compensation and as part of a regular business, issues or promulgates analyses or reports concerning securities"^^xsd:string ;
  rdfs:isDefinedBy <https://www.sec.gov/about/laws/iaa40.pdf> ;
  rdfs:label "US IAA Section 202(1)(11)"^^xsd:string ;
.
fo-iaa:Rule_Def_US_IAA_Sect_202a11_1_compensation
  rdf:type fo-fr:Legal_Rule ;
  fo-fr:applies_legal fo-iaa:inclusion_US_IAA_Section_202_1_11 ;
  rdfs:comment "‘‘Investment adviser’’ means any person who, for compensation, engages in the business of advising others, either directly or through publications or writings, as to the value of securities or as to the advisability of investing in, purchasing, or selling securities, or who, for compensation and as part of a regular business, issues or promulgates analyses or reports concerning securities"^^xsd:string ;
  rdfs:isDefinedBy <https://www.sec.gov/about/laws/iaa40.pdf> ;
  rdfs:label "US IAA Section 202(1)(11)"^^xsd:string ;
.
fo-iaa:Rule_Def_US_IAA_Sect_202a11_1_service
  rdf:type fo-fr:Legal_Rule ;
  fo-fr:applies_legal fo-iaa:inclusion_US_IAA_Section_202_1_11 ;
  rdfs:comment "‘‘Investment adviser’’ means any person who, for compensation, engages in the business of advising others, either directly or through publications or writings, as to the value of securities or as to the advisability of investing in, purchasing, or selling securities, or who, for compensation and as part of a regular business, issues or promulgates analyses or reports concerning securities"^^xsd:string ;
  rdfs:isDefinedBy <https://www.sec.gov/about/laws/iaa40.pdf> ;
  rdfs:label "US IAA Section 202(1)(11)"^^xsd:string ;
.
fo-iaa:Rule_Excl_US_IAA_Sect_202a11
  rdf:type fo-fr:Legal_Rule ;
  fo-fr:applies_legal fo-iaa:exclusion_US_IAA_Section_202_1_11 ;
  rdfs:comment "‘‘Investment adviser’’ means any person who, for compensation, engages in the business of advising others, either directly or through publications or writings, as to the value of securities or as to the advisability of investing in, purchasing, or selling securities, or who, for compensation and as part of a regular business, issues or promulgates analyses or reports concerning securities"^^xsd:string ;
  rdfs:isDefinedBy <https://www.sec.gov/about/laws/iaa40.pdf> ;
  rdfs:label "US IAA Section 202(1)(11)"^^xsd:string ;
.
fo-iaa:Rule_Excl_US_IAA_Sect_202a11_1_A_bank
  rdf:type fo-fr:Legal_Rule ;
  fo-fr:applies_legal fo-iaa:exclusion_US_IAA_Section_202_1_11 ;
  rdfs:comment "‘‘Investment adviser’’ means any person who, for compensation, engages in the business of advising others, either directly or through publications or writings, as to the value of securities or as to the advisability of investing in, purchasing, or selling securities, or who, for compensation and as part of a regular business, issues or promulgates analyses or reports concerning securities"^^xsd:string ;
  rdfs:isDefinedBy <https://www.sec.gov/about/laws/iaa40.pdf> ;
  rdfs:label "US IAA Section 202(1)(11)"^^xsd:string ;
.
fo-iaa:Rule_Excl_US_IAA_Sect_202a11_1_B_professional
  rdf:type fo-fr:Legal_Rule ;
  fo-fr:applies_legal fo-iaa:exclusion_US_IAA_Section_202_1_11 ;
  rdfs:comment "‘‘Investment adviser’’ means any person who, for compensation, engages in the business of advising others, either directly or through publications or writings, as to the value of securities or as to the advisability of investing in, purchasing, or selling securities, or who, for compensation and as part of a regular business, issues or promulgates analyses or reports concerning securities"^^xsd:string ;
  rdfs:isDefinedBy <https://www.sec.gov/about/laws/iaa40.pdf> ;
  rdfs:label "US IAA Section 202(1)(11)"^^xsd:string ;
.
fo-iaa:Rule_Excl_US_IAA_Sect_202a11_1_C_broker_dealer
  rdf:type fo-fr:Legal_Rule ;
  fo-fr:applies_legal fo-iaa:exclusion_US_IAA_Section_202_1_11 ;
  rdfs:comment "‘‘Investment adviser’’ means any person who, for compensation, engages in the business of advising others, either directly or through publications or writings, as to the value of securities or as to the advisability of investing in, purchasing, or selling securities, or who, for compensation and as part of a regular business, issues or promulgates analyses or reports concerning securities"^^xsd:string ;
  rdfs:isDefinedBy <https://www.sec.gov/about/laws/iaa40.pdf> ;
  rdfs:label "US IAA Section 202(1)(11)"^^xsd:string ;
.
fo-iaa:Rule_Excl_US_IAA_Sect_202a11_1_D_publisher
  rdf:type fo-fr:Legal_Rule ;
  fo-fr:applies_legal fo-iaa:exclusion_US_IAA_Section_202_1_11 ;
  rdfs:comment "‘‘Investment adviser’’ means any person who, for compensation, engages in the business of advising others, either directly or through publications or writings, as to the value of securities or as to the advisability of investing in, purchasing, or selling securities, or who, for compensation and as part of a regular business, issues or promulgates analyses or reports concerning securities"^^xsd:string ;
  rdfs:isDefinedBy <https://www.sec.gov/about/laws/iaa40.pdf> ;
  rdfs:label "US IAA Section 202(1)(11)"^^xsd:string ;
.
fo-iaa:Rule_Excl_US_IAA_Sect_202a11_1_E_gov_sec_only
  rdf:type fo-fr:Legal_Rule ;
  fo-fr:applies_legal fo-iaa:exclusion_US_IAA_Section_202_1_11 ;
  rdfs:comment "‘‘Investment adviser’’ means any person who, for compensation, engages in the business of advising others, either directly or through publications or writings, as to the value of securities or as to the advisability of investing in, purchasing, or selling securities, or who, for compensation and as part of a regular business, issues or promulgates analyses or reports concerning securities"^^xsd:string ;
  rdfs:isDefinedBy <https://www.sec.gov/about/laws/iaa40.pdf> ;
  rdfs:label "US IAA Section 202(1)(11)"^^xsd:string ;
.
fo-iaa:Rule_Excl_US_IAA_Sect_202a11_1_F_rating_organization
  rdf:type fo-fr:Legal_Rule ;
  fo-fr:applies_legal fo-iaa:exclusion_US_IAA_Section_202_1_11 ;
  rdfs:comment "‘‘Investment adviser’’ means any person who, for compensation, engages in the business of advising others, either directly or through publications or writings, as to the value of securities or as to the advisability of investing in, purchasing, or selling securities, or who, for compensation and as part of a regular business, issues or promulgates analyses or reports concerning securities"^^xsd:string ;
  rdfs:isDefinedBy <https://www.sec.gov/about/laws/iaa40.pdf> ;
  rdfs:label "US IAA Section 202(1)(11)"^^xsd:string ;
.
fo-iaa:Rule_Not_Excl_US_IAA_Sect_202a11
  rdf:type fo-fr:Legal_Rule ;
  fo-fr:applies_legal fo-iaa:inclusion_US_IAA_Section_202_1_11 ;
  rdfs:comment "‘‘Investment adviser’’ means any person who, for compensation, engages in the business of advising others, either directly or through publications or writings, as to the value of securities or as to the advisability of investing in, purchasing, or selling securities, or who, for compensation and as part of a regular business, issues or promulgates analyses or reports concerning securities"^^xsd:string ;
  rdfs:isDefinedBy <https://www.sec.gov/about/laws/iaa40.pdf> ;
  rdfs:label "US IAA Section 202(1)(11)"^^xsd:string ;
.
fo-iaa:Rule_US_IAA_Sect_202a11
  rdf:type fo-fr:Legal_Rule ;
  fo-fr:applies_legal fo-iaa:inclusion_US_IAA_Section_202_1_11 ;
  rdfs:comment "‘‘Investment adviser’’ means any person who, for compensation, engages in the business of advising others, either directly or through publications or writings, as to the value of securities or as to the advisability of investing in, purchasing, or selling securities, or who, for compensation and as part of a regular business, issues or promulgates analyses or reports concerning securities"^^xsd:string ;
  rdfs:isDefinedBy <https://www.sec.gov/about/laws/iaa40.pdf> ;
  rdfs:label "US IAA Section 202(1)(11)"^^xsd:string ;
.
fo-iaa:US_IAA
  rdf:type owl:Class ;
  rdfs:label "TD Prime Service"^^xsd:string ;
  rdfs:subClassOf <http://www.estrellaproject.org/lkif-core/norm.owl#Normatively_Qualified> ;
.
fo-iaa:exclusion_US_IAA_Section_202_1_11
  rdf:type fo-fr:Legal_Consequence ;
  rdfs:label "Inclusion under US IAA Section 202(1)(11)"^^xsd:string ;
.
fo-iaa:inclusion_US_IAA_Section_202_1_11
  rdf:type fo-fr:Legal_Consequence ;
  rdfs:label "Inclusion under US IAA Section 202(1)(11)"^^xsd:string ;
.
